# ãƒã‚¢ã‚½ãƒ³åˆ†å¸ƒ

## ç¢ºç‡è³ªé‡é–¢æ•°

```math
\begin{aligned}
p(k)=P(X=k) &= \binom{n}{k} p^k (1-p)^{n-k} \\
       &= \frac{n(n-1)\cdots(n-k+1)}{k!} \left( \frac{Î»}{n} \right)^k \left( 1 - \frac{Î»}{n} \right)^{n-k} \\
       &= \frac{Î»^k}{k!} \left( 1-\frac{1}{n} \right) \cdots \left( 1-\frac{k-1}{n} \right) \left( 1-\frac{Î»}{n} \right)^n \left( 1-\frac{Î»}{n} \right)^{-k} \\
       &\xrightarrow{nâ†’âˆ} \frac{Î»^k}{k!} (1-0) \cdots (1-0) e^{-Î»} (1-0)^{-k} \\
       &= e^{-Î»} \frac{Î»^k}{k!} \\
\end{aligned}
```

## ç¢ºç‡æ¯é–¢æ•°ãƒ»ç‰¹æ€§é–¢æ•°

```math
\begin{aligned}
G(s) = ğ”¼[s^X] &= \sum_{k=0}^âˆ s^k \cdot e^{-Î»} \frac{Î»^k}{k!} \\
              &= e^{-Î»} \sum_{k=0}^âˆ \frac{(sÎ»)^k}{k!} \\
              &= e^{-Î»} e^{sÎ»} \\
              &= e^{Î»(s-1)} \\
\end{aligned}
```

```math
\begin{equation}
Ï†(t) = G(e^{it}) = e^{Î»(e^{it}-1)}
\end{equation}
```

## å†ç”Ÿæ€§

ãƒã‚¢ã‚½ãƒ³åˆ†å¸ƒã«å¾“ã†ç‹¬ç«‹ãªç¢ºç‡å¤‰æ•°ã®å’Œã¯ã€ãƒã‚¢ã‚½ãƒ³åˆ†å¸ƒã«å¾“ã†ã€‚

```math
\begin{aligned}
X_1 \sim Po(Î»_1) \\
X_2 \sim Po(Î»_2) \\
Y = X_1 + X_2 \\
\end{aligned}
```

ä»¥ä¸Šã®å ´åˆã€

```math
\begin{aligned}
Ï†_Y(t) &= e^{Î»_1(e^{it}-1)} \cdot e^{Î»_2(e^{it}-1)} \\
       &= e^{(Î»_1 + Î»_2)(e^{it}-1)} \\
\end{aligned}
```

```math
\begin{equation}
\therefore Y \sim Po(Î»_1 + Î»_2)
\end{equation}
```

ã¨ãªã‚‹ã“ã¨ãŒåˆ†ã‹ã‚‹ã€‚
